Refactor Instrument.fst

io/model/Instrument.fst
@@ -1,27 +1,49 @@
 module Instrument
 
+open FStar.List
+open FStar.Tactics
+
 open Common
 open IO.Sig
 open DM
+open TC.Checkable
+open TC.Monitorable
+open TC.Instrumentable.IIO
+
+let rev_append_rev_append () : Lemma (
+  forall (h le1 le2:trace).
+    ((List.rev le2) @ (List.rev le1) @ h) ==
+      ((List.rev (le1@le2)) @ h))
+   by (FStar.Tactics.Derived.l_to_r [`List.append_assoc;`List.rev_append])
+      = ()
+
+let rec npnode (t:iio 'a) =
+  match t with
+  | Return _ -> True
+  | PartialCall _ _ -> False
+  | Call cmd arg fnc -> forall r. npnode (fnc r)
+  
+type npiio 'a = t:(iio 'a){npnode t}
 
 let rec _instrument
-  (tree : iio 'a)
-  ('p:monitorable_prop) :
+  (tree : npiio 'a)
+  ('p    : monitorable_prop)
+  (piprop:squash (forall h cmd arg. 'p cmd arg h ==> io_pre cmd arg h)) :
   IIOpi (maybe 'a) 'p (fun _ -> True) (fun _ _ _ -> True) =
   match tree with
   | Return r -> (Inl r)
   | Call GetTrace argz fnc ->
     let h = get_trace () in
-    let z' : iio 'a = fnc h in
-    rev_append_rev_append ();
-    _instrument z' 'p
+    let z' : npiio 'a = fnc h in
+    _instrument z' 'p piprop
   | Call cmd argz fnc -> begin
+    let d : checkable2 (io_pre cmd) = (
+      implies_is_checkable2 (io_sig.args cmd) trace ('p cmd) (io_pre cmd) piprop) in
     (** Check if the runtime check failed, and if yes, return the error **)
-    match dynamic_cmd cmd 'p argz with
+    match dynamic_cmd cmd d argz with
     | Inl rez ->
-      let z' : iio 'a = fnc rez in
-      rev_append_rev_append ();
-      _instrument z' 'p
+      let z' : npiio 'a = fnc rez in
+      _instrument z' 'p piprop
     | Inr err -> Inr err
   end
 
